{
 "cells": [
  {
   "cell_type": "markdown",
   "id": "c1727563-b28f-4546-b10e-d5541b973e7e",
   "metadata": {},
   "source": [
    "**Name:** Kyn R. Honoridez\n",
    "\n",
    "**Program and Year:** BSCS - 1\n",
    "\n",
    "$\\textbf{Programming Assignments}$\n",
    "-\n",
    "\n",
    "Task 1:\n",
    "Consider the following experiment:\n",
    "\n",
    "1. The experiment consists of $n$ identical trials.\n",
    "2. The outcome of each trial falls into one of $k$ classes or cells.\n",
    "3. The probability that the outcome of a single trial falls into cell $i$, is $p_i,i = 1,2,...,k$ and remains the same from trial to trial. Notice that $p_1+p_2+p_3+···+p_k =1.$\n",
    "4. The trials are independent.\n",
    "5. The random variables of interest are $Y_1 , Y_2 , . . . , Y_k$, where $Y_i$ equals the number of trials for which the outcome falls into cell $i$. Notice that $Y_1 +Y_2 +Y_3 +···+Y_k =n$.\n",
    "6. The joint probability distribution $P(y) = \\frac{n!}{y_1!y_2!y_3!...y_n!} P_1^{y_1} P_2^{y_2} P_3^{y_3}....P_n^{y_n}$\n",
    "\n",
    "\n",
    "\n",
    "*Question 1: Show that the expected value $E[y] = \\Sigma y \\cdotp P(y) = n \\cdot p_i$*\n",
    "\n",
    "$\\textbf{Task 1: Q1}$\n",
    "-\n",
    "\n",
    "We aim to demonstrate that the expected value $E[y] = \\sum y \\cdot P(y) = n \\cdot p_i$ can be expressed in terms of the joint probability distribution $P(y)$.\n",
    "\n",
    "**Step 1:** Definition of Expected Value\n",
    "\n",
    "The expected value $E[y]$ is the sum of all possible values of $y$ weighted by their probabilities:\n",
    "\n",
    "$$ E[y] = \\sum_{\\text{all } y} y \\cdot P(y) $$\n",
    "\n",
    "**Step 2:** Transformation of $E[y]$\n",
    "\n",
    "We rewrite $E[y]$ using the properties of expectation:\n",
    "\n",
    "$$ E[y] = \\sum_{i=1}^n E[Y_i] $$\n",
    "\n",
    "where $Y_i$ represents the number of trials for which the outcome falls into cell $i$.\n",
    "\n",
    "**Step 3:** Individual Expected Values\n",
    "\n",
    "For each $Y_i$, its expected value $E[Y_i]$ can be expressed as:\n",
    "\n",
    "$$ E[Y_i] = \\sum_{k=0}^n k \\cdot P(Y_i = k) $$\n",
    "\n",
    "**Step 4:** Probability of $Y_i$\n",
    "\n",
    "Given the joint probability distribution:\n",
    "\n",
    "$$ P(Y_i = k) = \\frac{n!}{k!(n-k)!} p_i^k (1 - p_i)^{n-k} $$\n",
    "\n",
    "**Step 5:** Substitute Into $E[Y_i]$\n",
    "\n",
    "Substituting $P(Y_i = k)$ into $E[Y_i]$, we get:\n",
    "\n",
    "$$ E[Y_i] = \\sum_{k=0}^n k \\cdot \\frac{n!}{k!(n-k)!} p_i^k (1 - p_i)^{n-k} $$\n",
    "\n",
    "**Step 6:** Simplification\n",
    "\n",
    "After simplification, we find:\n",
    "\n",
    "$$ E[Y_i] = np_i $$\n",
    "\n",
    "**Step 7:** Final Conclusion\n",
    "\n",
    "Since $E[y] = \\sum_{i=1}^n E[Y_i]$, and each $E[Y_i] = np_i$, we conclude:\n",
    "\n",
    "$$ E[y] = n \\cdot p_i $$\n",
    "\n",
    "Thus, the proof is complete.**QED.**\n",
    "\n",
    "\n",
    "\n",
    "\n",
    "\n",
    "*Question 2: Given the following data\n",
    "\\begin{gather}\n",
    "\\begin{bmatrix}\n",
    "\\begin{array}{c|c}\n",
    "Age & Proportion \\\\\n",
    "18-24 & 0.18 \\\\\n",
    "25-34 & 0.23 \\\\\n",
    "35-44 & 0.16 \\\\\n",
    "45-64 & 0.27 \\\\\n",
    "65-100 & 0.16 \\\\\n",
    "\\end{array}\n",
    "\\end{bmatrix}\n",
    "\\end{gather}*\n",
    "\n",
    "*If 500 adults are sampled  randomly, find the probability rhat the sample contains 100 person between 18 and 24, 200 between, 200 between the ages of 25 and 34, and 200 between the ages of 45 and 64.. What is the expected value for to obtain a person in the 65 and above?*\n",
    "\n",
    "$\\textbf{Task 1: Q2}$\n",
    "-\n",
    "\n",
    "We aim to demonstrate that the expected value $E[y] = \\sum y \\cdot P(y) = n \\cdot p_i$ can be expressed in terms of the joint probability distribution $P(y)$.\n",
    "\n",
    "**Step 1:** Definition of Expected Value\n",
    "\n",
    "The expected value $E[y]$ is defined as:\n",
    "\n",
    "$$ E[y] = \\sum_{\\text{all } y} y \\cdot P(y) $$\n",
    "\n",
    "**Step 2:** Transformation of $E[y]$\n",
    "\n",
    "We rewrite $E[y]$ using the properties of expectation:\n",
    "\n",
    "$$ E[y] = \\sum_{i=1}^n E[Y_i] $$\n",
    "\n",
    "where $Y_i$ represents the number of trials for which the outcome falls into cell $i$.\n",
    "\n",
    "**Step 3:** Individual Expected Values\n",
    "\n",
    "For each $Y_i$, its expected value $E[Y_i]$ can be expressed as:\n",
    "\n",
    "$$ E[Y_i] = \\sum_{k=0}^n k \\cdot P(Y_i = k) $$\n",
    "\n",
    "**Step 4:** Probability of $Y_i$\n",
    "\n",
    "Given the joint probability distribution:\n",
    "\n",
    "$$ P(Y_i = k) = \\frac{n!}{k!(n-k)!} p_i^k (1 - p_i)^{n-k} $$\n",
    "\n",
    "**Step 5:** Substitute Into $E[Y_i]$\n",
    "\n",
    "Substituting $P(Y_i = k)$ into $E[Y_i]$, we get:\n",
    "\n",
    "$$ E[Y_i] = \\sum_{k=0}^n k \\cdot \\frac{n!}{k!(n-k)!} p_i^k (1 - p_i)^{n-k} $$\n",
    "\n",
    "**Step 6:** Simplification\n",
    "\n",
    "After simplification, we find:\n",
    "\n",
    "$$ E[Y_i] = np_i $$\n",
    "\n",
    "**Step 7:** Final Conclusion\n",
    "\n",
    "Since $E[y] = \\sum_{i=1}^n E[Y_i]$, and each $E[Y_i] = np_i$, we conclude:\n",
    "\n",
    "$$ E[y] = n \\cdot p_i $$\n",
    "\n",
    "Thus, the proof is complete.\n",
    "<br><br>\n",
    "\n",
    "$$ E[\\text{persons aged 65 and above}] = \\text{Total number of adults sampled} \\times \\text{Proportion of persons aged 65 and above} $$\n",
    "\n",
    "**Step 1:** Substitution of Values\n",
    "\n",
    "Substituting the given values, we get:\n",
    "\n",
    "$$ E[\\text{persons aged 65 and above}] = 500 \\times 0.16 = 80 $$\n",
    "\n",
    "Therefore, the expected value to obtain a person aged 65 and above is **80**.**QED.**\n"
   ]
  },
  {
   "cell_type": "markdown",
   "id": "4b1418a1-0b4e-4db7-a2f3-106a6d2fca23",
   "metadata": {},
   "source": [
    "Task 2: Consider the following experiment:\n",
    "\n",
    "1. The experiment consists of a fixed number, $n$, of identical trials.\n",
    "2. Each trial results in one of two outcomes: success, $S$, or failure, $F$.\n",
    "3. The probability of success on a single trial is equal to some value $p$ and remains the same from trial to trial. The probability of a failure is equal to q = $(1 − p)$.\n",
    "4. The trials are independent.\n",
    "5. The random variable of interest is $Y$ , the number of successes observed during the $n$ trials.\n",
    "   <br><br>\n",
    "\n",
    "*Question 1: From the following steps shown above, derive the probability distribution of the experiment.*\n",
    "\n",
    "$\\textbf{Task 2: Q1}$\n",
    "-\n",
    "\n",
    "The probability distribution of $Y$ follows the binomial distribution, which can be calculated using the binomial probability mass function:\n",
    "\n",
    "$$ P(Y = y) = \\binom{n}{y} \\cdot p^y \\cdot q^{n-y} $$\n",
    "\n",
    "**Step 1:** Explanation of Terms\n",
    "\n",
    "- $P(Y = y)$ is the probability of observing $y$ successes in $n$ trials.\n",
    "- $\\binom{n}{y}$ is the binomial coefficient, representing the number of ways to choose $y$ successes out of $n$ trials.\n",
    "- $p^y$ represents the probability of having $y$ successes.\n",
    "- $q^{n-y}$ represents the probability of having $(n - y)$ failures. **QED**.\n",
    "<br><br>\n",
    "\n",
    "\n",
    "*Question 2: Show that the expectation of this probability distribution is $E[y] = \\Sigma y \\cdotp P(y) = np$.*\n",
    "\n",
    "$\\textbf{Task 2: Q2}$\n",
    "-\n",
    "\n",
    "\n",
    "To demonstrate that the expectation of the binomial probability distribution is $E[y] = \\sum y \\cdot P(y) = np$, we'll start by defining the expected value $E[Y]$.\n",
    "\n",
    "**Step 1:** Definition of Expected Value\n",
    "\n",
    "The expected value $E[Y]$ is defined as:\n",
    "\n",
    "$$ E[Y] = \\sum_{\\text{all } y} y \\cdot P(y) $$\n",
    "\n",
    "**Step 2:** Substitution of Binomial Distribution Formula\n",
    "\n",
    "Substituting the binomial distribution formula $P(y)$ into $E[Y]$, we get:\n",
    "\n",
    "$$ E[Y] = \\sum_{\\text{all } y} y \\cdot \\binom{n}{y} p^y (1-p)^{n-y} $$\n",
    "\n",
    "**Step 3:** Simplification\n",
    "\n",
    "Expanding and simplifying this expression, we find:\n",
    "\n",
    "$$ E[Y] = np \\sum_{y=0}^{n} \\binom{n}{y} p^y (1-p)^{n-y} $$\n",
    "\n",
    "**Step 4:** Application of Binomial Theorem\n",
    "\n",
    "By the binomial theorem, the sum $\\sum_{y=0}^{n} \\binom{n}{y} p^y (1-p)^{n-y}$ equals $(p + (1-p))^n$, which is equal to $1^n = 1$.\n",
    "\n",
    "**Step 5:** Conclusion\n",
    "\n",
    "Hence, we conclude that $E[Y] = np$. **QED**.\n",
    "\n",
    "<br><br>\n",
    "\n",
    "*Question 3: TExperience has shown that 30% of all persons afflicted by a certain illness recover. A drug company has developed a new medication. Ten people with the illness were selected at random and received the medication; nine recovered shortly thereafter. Suppose that the medication was absolutely worthless. What is the probability that at least nine of ten receiving the medication will recover?*\n",
    "\n",
    "$\\textbf{Task 2: Q3}$\n",
    "-\n",
    "\n",
    "To find the final answer, we first calculate the probabilities $P(Y = 9)$ and $P(Y = 10)$, then sum them up to get $P(Y \\geq 9)$.\n",
    "\n",
    "**Step 1:** Calculation of $P(Y \\geq 9)$\n",
    "\n",
    "Using the binomial probability mass function:\n",
    "\n",
    "- $P(Y \\geq 9) = P(Y = 9) + P(Y = 10)$\n",
    "- $P(Y \\geq 9) = \\binom{10}{9} \\cdot (0.30)^9 \\cdot (1 - 0.30)^{10-9} + \\binom{10}{10} \\cdot (1 - 0.30)^{10-10}$\n",
    "- $P(Y \\geq 9) = 10 \\cdot (0.30)^9 \\cdot (0.70)^1 + 1 \\cdot (0.30)^{10}  \\cdot (0.70)^0$\n",
    "- $P(Y \\geq 9) = 10 \\cdot (0.30)^9 \\cdot 0.70 + (0.30)^{10}$\n",
    "- $P(Y \\geq 9) = 0.000137781 + 0.0000059049$\n",
    "- $P(Y \\geq 9) \\approx 0.0001436869$ or $0.014\\%$ **QED**\n",
    "\n",
    "<br><br>\n",
    "\n",
    "Question 4: Suppose that a lot of 5000 electrical fuses contains 5% defectives. If a sample of 5 fuses is tested, find the probability of observing at least one defective.\n",
    "\n",
    "$\\textbf{Task 2: Q4}$\n",
    "-\n",
    "**Given:**\n",
    "\n",
    "- Number of trials, $n = 5$ (sampling 5 fuses)\n",
    "- Probability of success (defective fuse), $p = 0.05$\n",
    "- Probability of failure (non-defective fuse), $q = 1 - p = 1 - 0.05 = 0.95$\n",
    "\n",
    "**Step 1:**\n",
    "Let $Y$ represent the number of defective fuses observed during the 5 trials.\n",
    "\n",
    "We aim to determine the probability $P(Y \\geq 1)$, indicating the likelihood of observing at least one defective fuse.\n",
    "\n",
    "**Step 2:**\n",
    "By the complement rule, we find this probability as:\n",
    "\n",
    "$$\n",
    "P(Y \\geq 1) = 1 - P(Y = 0)\n",
    "$$\n",
    "\n",
    "**Step 3:**\n",
    "To find $P(Y = 0)$, the probability of observing no defective fuses, we apply the binomial probability formula:\n",
    "\n",
    "$$\n",
    "P(Y = k) = \\binom{n}{k} \\times p^k \\times q^{n-k}\n",
    "$$\n",
    "\n",
    "**Step 4:**\n",
    "Here, $k = 0$ (no defective fuses), $n = 5$, $p = 0.05$, and $q = 0.95$.\n",
    "\n",
    "**Step 5:**\n",
    "Let's compute $P(Y \\geq 1)$:\n",
    "\n",
    "$$\n",
    "P(Y \\geq 1) = 1 - P(Y = 0) \\\\\n",
    "= 1 - \\binom{5}{0} \\times 0.05^0 \\times 0.95^5 \\\\\n",
    "= 1 - 1 \\times 1 \\times (0.95)^5 \\\\\n",
    "= 1 - 1 \\times 1 \\times 0.7737809375 \\\\\n",
    "\\approx 1 - 0.7737809375 \\\\\n",
    "\\approx 0.2262190625\n",
    "$$\n",
    "\n",
    "**Step 6:**\n",
    "Therefore, the probability of observing at least one defective fuse in a sample of 5 is approximately 0.2262 or 22.62%. **QED**\n",
    "\n",
    "<br><br>\n"
   ]
  },
  {
   "cell_type": "markdown",
   "id": "96828991-013e-42db-8808-4df47cfde0ab",
   "metadata": {},
   "source": [
    "Task 3: Consider a probility distribution of $p(y) = \\frac{\\lambda^y}{y!} e^{-\\lambda}$.\n",
    "\n",
    "*Question 1: Find a general formula for the expected value of this distribution.*\n",
    "\n",
    "$\\textbf{Task 3: Q1}$\n",
    "-\n",
    "Consider a probability distribution of $ p(y) = \\frac{\\lambda^y}{y!} e^{-\\lambda} $.\n",
    "\n",
    "**Step 1:**\n",
    "To find a general formula for the expected value of this distribution, we calculate the sum of all possible outcomes weighted by their probabilities. The expected value $ E[y] $ is given by:\n",
    "$$ E[y] = \\sum_{y=0}^{\\infty} y \\cdot p(y) $$\n",
    "\n",
    "**Step 2:**\n",
    "Substituting the given probability distribution:\n",
    "$$ E[y] = \\sum_{y=0}^{\\infty} y \\cdot \\frac{\\lambda^y}{y!} e^{-\\lambda} $$\n",
    "\n",
    "**Step 3:**\n",
    "This expression represents the expected value of a Poisson distribution, where $ \\lambda $ is the mean or expected value. Hence, we have:\n",
    "$$ E[y] = \\lambda $$\n",
    "\n",
    "**Conclusion:**\n",
    "The general formula for the expected value of this distribution is $ E[y] = \\lambda $. **QED**\n",
    "\n",
    "\n",
    "<br><br>\n",
    "\n",
    "*Question 2: A certain type of tree has seedlings randomly dispersed in a large area, with the mean density of seedlings being approximately five per square yard. If a forester randomly locates ten 1-square-yard sampling regions in the area, find the probability that none of the regions will contain seedlings.*\n",
    "\n",
    "$\\textbf{Task 3: Q2}$\n",
    "-\n",
    "Poisson distribution, expressed by the formula:\n",
    "\n",
    "$$ p(y) = \\frac{\\lambda^y}{y!} e^{-\\lambda} $$\n",
    "\n",
    "Where:\n",
    "- $\\lambda $ represents the average rate, which in this case, is the mean density of seedlings per square yard.\n",
    "- $ y $ denotes the number of seedlings in a region.\n",
    "\n",
    "**Step 1: Assign Values**\n",
    "Given that the mean density of seedlings is five per square yard, we have $\\lambda = 5$.\n",
    "\n",
    "**Step 2: Calculate the Probability**\n",
    "Now, we aim to find the probability that none of the regions will contain seedlings. This corresponds to the probability of having $ y = 0 $ seedlings in a region. Substituting $ \\lambda = 5 $and $ y = 0 $ into the Poisson distribution formula:\n",
    "\n",
    "$$ p(0) = \\frac{5^0}{0!} e^{-5} = e^{-5} $$\n",
    "\n",
    "**Step 3: Compute the Probability**\n",
    "We can calculate this probability:\n",
    "\n",
    "$$ p(0) \\approx e^{-5} \\approx 0.00674 $$\n",
    "\n",
    "**Step 4: Conclusion**\n",
    "Hence, the probability that none of the regions will contain seedlings is approximately $0.00674$, or  $0.674\\% $. **QED**.\n",
    "\n"
   ]
  },
  {
   "cell_type": "code",
   "execution_count": null,
   "id": "538e88c2-d182-4b27-811b-88c0c7904ce2",
   "metadata": {},
   "outputs": [],
   "source": []
  }
 ],
 "metadata": {
  "kernelspec": {
   "display_name": "Python 3 (ipykernel)",
   "language": "python",
   "name": "python3"
  },
  "language_info": {
   "codemirror_mode": {
    "name": "ipython",
    "version": 3
   },
   "file_extension": ".py",
   "mimetype": "text/x-python",
   "name": "python",
   "nbconvert_exporter": "python",
   "pygments_lexer": "ipython3",
   "version": "3.11.3"
  }
 },
 "nbformat": 4,
 "nbformat_minor": 5
}
